Regex/Data/Parsec/Basic.lean
@@ -7,126 +7,126 @@ open Lean Lean.Syntax Parser Parser.Char
 namespace Parser
 
 instance Parser.coeSimpleParser
-    : Coe ((SimpleParser Substring Char) α) ((ReaderT ρ $ StateT σ (SimpleParser Substring Char)) α) where
+    : Coe ((SimpleParser Substring.Raw Char) α) ((ReaderT ρ $ StateT σ (SimpleParser Substring.Raw Char)) α) where
   coe p := fun _ σ => do return (← p, σ)
 
 /-- extends `Lean.Parser.attempt` -/
-def attemptM (p : (ReaderT ρ $ StateT σ (SimpleParser Substring Char)) α)
-    : (ReaderT ρ $ StateT σ (SimpleParser Substring Char)) α := fun f => do
+def attemptM (p : (ReaderT ρ $ StateT σ (SimpleParser Substring.Raw Char)) α)
+    : (ReaderT ρ $ StateT σ (SimpleParser Substring.Raw Char)) α := fun f => do
   let (a, s) ← Parser.withBacktracking (p f (← get))
   set s
   pure a
 
-def fail (msg : String) : (SimpleParser Substring Char) α :=
+def fail (msg : String) : (SimpleParser Substring.Raw Char) α :=
   throwUnexpectedWithMessage none msg
 
-private def orElseT (p : (SimpleParser Substring Char) α)
-  (q : Unit → (ReaderT ρ $ StateT σ (SimpleParser Substring Char)) α)
-    : (ReaderT ρ $ StateT σ (SimpleParser Substring Char)) α := λ f s => do
+private def orElseT (p : (SimpleParser Substring.Raw Char) α)
+  (q : Unit → (ReaderT ρ $ StateT σ (SimpleParser Substring.Raw Char)) α)
+    : (ReaderT ρ $ StateT σ (SimpleParser Substring.Raw Char)) α := λ f s => do
   match ← eoption p with
   | .inl x => return (x, s)
   | .inr _ => (q ()) f s
 
 instance : HOrElse
-    ((SimpleParser Substring Char) α) ((ReaderT ρ $ StateT σ (SimpleParser Substring Char)) α)
-    ((ReaderT ρ $ StateT σ (SimpleParser Substring Char)) α) where
+    ((SimpleParser Substring.Raw Char) α) ((ReaderT ρ $ StateT σ (SimpleParser Substring.Raw Char)) α)
+    ((ReaderT ρ $ StateT σ (SimpleParser Substring.Raw Char)) α) where
   hOrElse := orElseT
 
-partial def manyCore (p : (SimpleParser Substring Char) α)
-  (acc : Array α) : (SimpleParser Substring Char) $ Array α := do
+partial def manyCore (p : (SimpleParser Substring.Raw Char) α)
+  (acc : Array α) : (SimpleParser Substring.Raw Char) $ Array α := do
   let r ← Parser.efoldl (fun arr x => arr.push x) acc (Parser.withBacktracking p)
   return r.1
 
-private def tryCatchT (p : StateT σ (SimpleParser Substring Char) α)
-    (csuccess : α → StateT σ (SimpleParser Substring Char) α')
-    (cerror : Unit → StateT σ (SimpleParser Substring Char) α')
-    : StateT σ  (SimpleParser Substring Char) α' := fun s it =>
+private def tryCatchT (p : StateT σ (SimpleParser Substring.Raw Char) α)
+    (csuccess : α → StateT σ (SimpleParser Substring.Raw Char) α')
+    (cerror : Unit → StateT σ (SimpleParser Substring.Raw Char) α')
+    : StateT σ  (SimpleParser Substring.Raw Char) α' := fun s it =>
   match withBacktracking (p s) it with
   | .ok rem a => csuccess a.1 a.2 rem
   | .error rem _ => cerror () s rem
 
-private partial def manyCoreT (p : StateT σ (SimpleParser Substring Char) α)
+private partial def manyCoreT (p : StateT σ (SimpleParser Substring.Raw Char) α)
   (acc : Array α)
-    : StateT σ (SimpleParser Substring Char) $ Array α :=
+    : StateT σ (SimpleParser Substring.Raw Char) $ Array α :=
   tryCatchT p (manyCoreT p <| acc.push ·) (fun _ => pure acc)
 
 /-- extends `Lean.Parser.many` -/
-partial def manyM (p : (ReaderT ρ $ StateT σ (SimpleParser Substring Char)) α)
-    : (ReaderT ρ $ StateT σ (SimpleParser Substring Char)) $ Array α := do
+partial def manyM (p : (ReaderT ρ $ StateT σ (SimpleParser Substring.Raw Char)) α)
+    : (ReaderT ρ $ StateT σ (SimpleParser Substring.Raw Char)) $ Array α := do
   manyCoreT (p (← read)) #[]
 
-def ws : (ReaderT ρ $ StateT σ (SimpleParser Substring Char)) PUnit := fun _ t => do
+def ws : (ReaderT ρ $ StateT σ (SimpleParser Substring.Raw Char)) PUnit := fun _ t => do
   let _ ← manyCore (Char.ASCII.whitespace) #[]
   pure ((), t)
 
-def peekChar?  : (SimpleParser Substring Char) $ Option Char := do
+def peekChar?  : (SimpleParser Substring.Raw Char) $ Option Char := do
   match ← eoption peek with
   | .inl x => return some x
   | .inr _ => return none
 
-def peekChar : (SimpleParser Substring Char) Char :=
+def peekChar : (SimpleParser Substring.Raw Char) Char :=
   peek
 
-def withPos (p : (SimpleParser Substring Char) α)
-    : (SimpleParser Substring Char) (String.Pos.Raw × String.Pos.Raw × α) := do
+def withPos (p : (SimpleParser Substring.Raw Char) α)
+    : (SimpleParser Substring.Raw Char) (String.Pos.Raw × String.Pos.Raw × α) := do
   let cap ← Char.captureStr p
   return (cap.2.startPos, cap.2.stopPos, cap.1)
 
-def withPosM (p : (ReaderT ρ $ StateT σ (SimpleParser Substring Char)) α)
-    : (ReaderT ρ $ StateT σ (SimpleParser Substring Char)) (String.Pos.Raw × String.Pos.Raw × α) := fun f s => do
+def withPosM (p : (ReaderT ρ $ StateT σ (SimpleParser Substring.Raw Char)) α)
+    : (ReaderT ρ $ StateT σ (SimpleParser Substring.Raw Char)) (String.Pos.Raw × String.Pos.Raw × α) := fun f s => do
   let cap ← Char.captureStr (p f s)
   return ((cap.2.startPos, cap.2.stopPos, cap.1.1), cap.1.2)
 
-def withPosSkip : (SimpleParser Substring Char) String.Pos.Raw := do
+def withPosSkip : (SimpleParser Substring.Raw Char) String.Pos.Raw := do
   let (_, t, _) ← withPos anyToken
   pure t
 
 
-def skipChar (c : Char) : (SimpleParser Substring Char) Unit := do
+def skipChar (c : Char) : (SimpleParser Substring.Raw Char) Unit := do
   match ← eoption peek with
   | .inl c' => if c = c' then anyToken *> pure () else throwUnexpected
   | .inr e => throw e
 
-def skipAnyChar : (SimpleParser Substring Char) Unit := do
+def skipAnyChar : (SimpleParser Substring.Raw Char) Unit := do
   anyToken *> pure ()
 
-def skipChar? (c : Char) : (SimpleParser Substring Char) Unit := do
+def skipChar? (c : Char) : (SimpleParser Substring.Raw Char) Unit := do
   try skipChar c
   catch _ => pure ()
 
-def skipString (tks : String) : (SimpleParser Substring Char) Unit := do
+def skipString (tks : String) : (SimpleParser Substring.Raw Char) Unit := do
   string tks *> pure ()
 
-def skipString? (tks : String) : (SimpleParser Substring Char) Unit := do
+def skipString? (tks : String) : (SimpleParser Substring.Raw Char) Unit := do
   try withBacktracking (skipString tks)
   catch _ => pure ()
 
 /-- exec `check` on current char -/
-def testChar (check : Char -> Bool) : (SimpleParser Substring Char) Bool := do
+def testChar (check : Char -> Bool) : (SimpleParser Substring.Raw Char) Bool := do
   match ← peekChar? with
   | some c => if check c then pure true else pure false
   | none => pure false
 
 /-- exec `check` on current char and consume char on success -/
-def tryChar (check : Char -> Bool) : (SimpleParser Substring Char) $ Option Char := do
+def tryChar (check : Char -> Bool) : (SimpleParser Substring.Raw Char) $ Option Char := do
   match ← peekChar? with
   | some c => if check c then pure $ some (← anyToken) else pure none
   | none => pure none
 
 /-- exec `check` on current char and skip char on success -/
-def trySkipChar (check : Char -> Bool) : (SimpleParser Substring Char) Bool := do
+def trySkipChar (check : Char -> Bool) : (SimpleParser Substring.Raw Char) Bool := do
   if let some _ ← tryChar check then pure true else pure false
 
 /-- exec `check` on current char and then exec `p` on success -/
-def tryCharThenPWithPos (check : Char -> Bool) (p : (SimpleParser Substring Char) α)
-    : (SimpleParser Substring Char) $ Option (String.Pos.Raw × String.Pos.Raw × α) := do
+def tryCharThenPWithPos (check : Char -> Bool) (p : (SimpleParser Substring.Raw Char) α)
+    : (SimpleParser Substring.Raw Char) $ Option (String.Pos.Raw × String.Pos.Raw × α) := do
   match ← peekChar? with
   | some c => if check c then pure $ some (← withPos p) else pure none
   | none => pure none
 
 /-- exec `check` on current char and then exec `p` on success -/
-def tryCharThenPWithPosM (check : Char -> Bool) (p : (ReaderT ρ $ StateT σ (SimpleParser Substring Char)) α)
-    : (ReaderT ρ $ StateT σ (SimpleParser Substring Char)) $ Option (String.Pos.Raw × String.Pos.Raw × α) := fun f s => do
+def tryCharThenPWithPosM (check : Char -> Bool) (p : (ReaderT ρ $ StateT σ (SimpleParser Substring.Raw Char)) α)
+    : (ReaderT ρ $ StateT σ (SimpleParser Substring.Raw Char)) $ Option (String.Pos.Raw × String.Pos.Raw × α) := fun f s => do
   match ← peekChar? with
   | some c => if check c then
                 let x ← withPos (p f s)
@@ -135,18 +135,18 @@ def tryCharThenPWithPosM (check : Char -> Bool) (p : (ReaderT ρ $ StateT σ (Si
   | none => pure (none, s)
 
 def tryCharWithPos (check : Char -> Bool)
-    :  (SimpleParser Substring Char) $ Option (String.Pos.Raw × String.Pos.Raw × Char) := do
+    :  (SimpleParser Substring.Raw Char) $ Option (String.Pos.Raw × String.Pos.Raw × Char) := do
   tryCharThenPWithPos check anyToken
 
 def tryCharWithPosMap (check : Char -> Bool) (f : Char → String.Pos.Raw → String.Pos.Raw → α)
-    :  (SimpleParser Substring Char) $ Option α := do
+    :  (SimpleParser Substring.Raw Char) $ Option α := do
   if let some (p1, p2, c) ← tryCharWithPos check then pure $ f c p1 p2
   else pure none
 
-def manyChars (p : (SimpleParser Substring Char) Char) : (SimpleParser Substring Char) String := do
+def manyChars (p : (SimpleParser Substring.Raw Char) Char) : (SimpleParser Substring.Raw Char) String := do
   let chars ← manyCore p #[]
-  return chars.toList.asString
+  return String.ofList chars.toList
 
-def many1Chars (p : (SimpleParser Substring Char) Char) : (SimpleParser Substring Char) String := do
+def many1Chars (p : (SimpleParser Substring.Raw Char) Char) : (SimpleParser Substring.Raw Char) String := do
   let chars ← manyCore p #[← p]
-  return chars.toList.asString
+  return String.ofList chars.toList
