Regex/Unicode/Utils.lean
@@ -4,7 +4,7 @@ import Regex.Interval
 namespace Unicode
 
 /-- extract data from records -/
-def extract (data : Array (Array Substring)) : Array (String × UInt32 × (Option UInt32)) :=
+def extract (data : Array (Array Substring.Raw)) : Array (String × UInt32 × (Option UInt32)) :=
   let init : Array (String × UInt32 × (Option UInt32)) := #[]
   data |> Array.foldl (init := init) (fun acc record =>
     let val : UInt32 × Option UInt32 :=
